Frame and anti frame + abrupt + hoare rule for recursive prog
git-svn-id: orca@542

C-verifier/src/Midend-IVL/Isabelle-UTP-Extended/hoare/HoareLogic/TotalCorrectness/IMP_Prog/utp_hoare_ndes_prog.thy
@@ -1,6 +1,7 @@
 theory utp_hoare_ndes_prog
 
-imports "../../../../impl/utp_prog_des_more"
+  imports "../../../../impl/utp_prog_des_more"
+          "../../../AlgebraicLaws/IMP_Prog/algebraic_laws_prog"
 
 begin
 section {*Hoare logic for designs*}  
@@ -91,269 +92,48 @@ lemma cond_d_hoare_d_t [hoare_prog]:
 
 subsection {*Hoare for recursion*}
 
+lemma mono_Monotone_prog: (*This can be used to generate lemmas automatically*)
+  assumes M:"mono F" 
+  shows "Mono\<^bsub>uthy_order NDES\<^esub> (Rep_prog \<circ> F \<circ> Abs_prog \<circ> \<H>\<^bsub>NDES\<^esub>)"
+  by (metis (no_types, lifting) Abs_prog_Rep_prog_Ncarrier Healthy_def M Mono_utp_orderI comp_apply less_eq_prog.rep_eq monoD)
+
+lemma N_prog_funcset: (*This can be used to generate lemmas automatically*)
+  "Rep_prog \<circ> F \<circ> Abs_prog \<circ> \<H>\<^bsub>NDES\<^esub> \<in> \<lbrakk>\<^bold>N\<rbrakk>\<^sub>H \<rightarrow> \<lbrakk>\<^bold>N\<rbrakk>\<^sub>H"  
+  using Rep_prog by auto
+   
 lemma mu_p_rec_hoare_p_t [hoare_prog]:
   assumes WF: "wf R"
-  assumes M:"mono (Rep_prog o F)"  
+  assumes M:"mono F"  
   assumes induct_step:
     "\<And> st P. \<lbrace>Pre \<and>(E,\<guillemotleft>st\<guillemotright>)\<^sub>u\<in>\<^sub>u\<guillemotleft>R\<guillemotright>\<rbrace> P \<lbrace>Post\<rbrace>\<^sub>P \<Longrightarrow> \<lbrace>Pre \<and> E =\<^sub>u \<guillemotleft>st\<guillemotright>\<rbrace> F P \<lbrace>Post\<rbrace>\<^sub>P"   
   shows "\<lbrace>Pre\<rbrace>\<mu>\<^sub>p F \<lbrace>Post\<rbrace>\<^sub>P"
   apply (simp add: prog_rep_eq)
   apply (subst normal_design_theory_continuous.LFP_healthy_comp)  
-  apply (rule mu_p_rec_hoare_p_t[OF WF, of _ _ E])
-    apply (metis (no_types, lifting) Abs_prog_Rep_prog_Ncarrier Healthy_def M Mono_utp_orderI comp_apply less_eq_prog.rep_eq monoD)
-  using Rep_prog apply fastforce
+  apply (rule mu_d_rec_hoare_d_t[OF WF mono_Monotone_prog[OF M] N_prog_funcset, 
+                                    simplified, OF induct_step[unfolded prog_rep_eq]])
   apply (simp add: Abs_prog_Rep_prog_Ncarrier)   
-  apply (rule induct_step[unfolded prog_rep_eq])
-  apply (simp add: Abs_prog_Rep_prog_Ncarrier)
   apply (simp add: Healthy_if is_Ncarrier_is_ndesigns)
   done
     
 lemma mu_p_rec_hoare_p_t' [hoare_prog]:
   assumes WF: "wf R"
-  assumes M:"mono (Rep_prog o F)"  
+  assumes M:"mono F"  
   assumes induct_step:
     "\<And> st P. \<lbrace>Pre \<and>(E,\<guillemotleft>st\<guillemotright>)\<^sub>u\<in>\<^sub>u\<guillemotleft>R\<guillemotright>\<rbrace> P \<lbrace>Post\<rbrace>\<^sub>P \<Longrightarrow> \<lbrace>Pre \<and> E =\<^sub>u \<guillemotleft>st\<guillemotright>\<rbrace> F P \<lbrace>Post\<rbrace>\<^sub>P" 
   assumes I0: "`Pre' \<Rightarrow> Pre`"  
   shows "\<lbrace>Pre'\<rbrace>\<mu>\<^sub>p F \<lbrace>Post\<rbrace>\<^sub>P"
-  apply (rule hoare_pre_str_d_t[OF I0])
-  apply (rule mu_p_rec_hoare_p_t[OF WF M induct_step])
-  apply assumption
-  done
+  by (simp add: hoare_pre_str_d_t[OF I0 mu_p_rec_hoare_p_t[OF WF M induct_step]])
 
 subsection {*Hoare for while iteration*}   
 
 lemma while_hoare_p_t [hoare_prog]:
   assumes WF: "wf R"
   assumes I0: "`Pre \<Rightarrow> I`" 
-  assumes induct_step:"\<And> st. \<lbrace>b \<and> I \<and> E =\<^sub>u \<guillemotleft>st\<guillemotright>\<rbrace> body \<lbrace>I \<and>(E,\<guillemotleft>st\<guillemotright>)\<^sub>u\<in>\<^sub>u\<guillemotleft>R\<guillemotright>\<rbrace>\<^sub>P"  
+  assumes induct_step:"\<And>e. \<lbrace>b \<and> I \<and> E =\<^sub>u \<guillemotleft>e\<guillemotright>\<rbrace> body \<lbrace>I \<and>(E,\<guillemotleft>e\<guillemotright>)\<^sub>u\<in>\<^sub>u\<guillemotleft>R\<guillemotright>\<rbrace>\<^sub>P"  
   assumes PHI:"`(\<not> b \<and> I) \<Rightarrow> Post`"  
   shows "\<lbrace>Pre\<rbrace>INVR I WHILE b DO body OD \<lbrace>Post\<rbrace>\<^sub>P"
   unfolding pwhile_inv_prog_def
   by (simp add: prog_rep_eq while_hoare_ndesign_t[unfolded While_inv_ndes_def, OF WF I0  Rep_prog_H1_H3_closed[THEN H1_H3_impl_H2, THEN H1_H2_impl_H1] induct_step[unfolded prog_rep_eq] PHI])
 
-section {*Abrupt*}
-subsection {*Sequential C-program alphabet*}
 
-text 
-{* In order to capture exceptions, we extend the alphabet of UTP by an additional global 
-   state variables:
-   \begin{itemize}   
-      \<^item> abrupt: a boolean variable used to specify if the program is in an abrupt state or not.
-   \end{itemize}
-*}
-
-alphabet abr_vars = 
-  abrupt :: bool
-
-declare  abr_vars.splits [alpha_splits]
-  
-subsubsection {*Alphabet proofs*}
-text {*
-  The two locale interpretations below are a technicality to improve automatic
-  proof support via the predicate and relational tactics. This is to enable the
-  (re-)interpretation of state spaces to remove any occurrences of lens types
-  after the proof tactics @{method pred_simp} and @{method rel_simp}, or any
-  of their derivatives have been applied. Eventually, it would be desirable to
-  automate both interpretations as part of a custom outer command for defining
-  alphabets.
-*}
-
-interpretation cp_abr:
-  lens_interp "\<lambda> (ok, r) . (ok, abrupt\<^sub>v r, more r)"
-apply (unfold_locales)
-apply (rule injI)
-apply (clarsimp)
-done
-
-interpretation cp_abr_rel: lens_interp "\<lambda>(ok, ok', r, r').
-  (ok, ok', abrupt\<^sub>v r, abrupt\<^sub>v r', more r, more r')"
-apply (unfold_locales)
-apply (rule injI)
-apply (clarsimp)
-done
-
-subsubsection {*Type lifting*}
-
-type_synonym '\<alpha> hrel_abr_des  = "'\<alpha> abr_vars_scheme prog"
-
-subsubsection {*Syntactic type setup*}
-
-notation abr_vars_child_lens ("\<Sigma>\<^sub>A\<^sub>B\<^sub>R")
-
-syntax
-  "_svid_st_alpha"  :: "svid" ("\<Sigma>\<^sub>A\<^sub>B\<^sub>R")
-translations
-  "_svid_st_alpha" => "CONST abr_vars_child_lens"
-
-subsection {*Substitution lift and drop*}
-
-abbreviation lift_rel_usubst_cpa ("\<lceil>_\<rceil>\<^sub>S\<^sub>A\<^sub>B\<^sub>R")
-where "\<lceil>\<sigma>\<rceil>\<^sub>S\<^sub>A\<^sub>B\<^sub>R \<equiv> \<sigma> \<oplus>\<^sub>s (\<Sigma>\<^sub>A\<^sub>B\<^sub>R \<times>\<^sub>L \<Sigma>\<^sub>A\<^sub>B\<^sub>R)"
-
-abbreviation lift_usubst_cpa ("\<lceil>_\<rceil>\<^sub>s\<^sub>A\<^sub>B\<^sub>R")
-where "\<lceil>\<sigma>\<rceil>\<^sub>s\<^sub>A\<^sub>B\<^sub>R \<equiv> \<lceil>\<lceil>\<sigma>\<rceil>\<^sub>s\<rceil>\<^sub>S\<^sub>A\<^sub>B\<^sub>R"
-
-abbreviation drop_cpa_rel_usubst ("\<lfloor>_\<rfloor>\<^sub>S\<^sub>A\<^sub>B\<^sub>R")
-where "\<lfloor>\<sigma>\<rfloor>\<^sub>S\<^sub>A\<^sub>B\<^sub>R \<equiv> \<sigma> \<restriction>\<^sub>s (\<Sigma>\<^sub>A\<^sub>B\<^sub>R \<times>\<^sub>L \<Sigma>\<^sub>A\<^sub>B\<^sub>R)"
-
-abbreviation drop_cpa_usubst ("\<lfloor>_\<rfloor>\<^sub>s\<^sub>A\<^sub>B\<^sub>R")
-where "\<lfloor>\<sigma>\<rfloor>\<^sub>s\<^sub>A\<^sub>B\<^sub>R \<equiv> \<lfloor>\<lfloor>\<sigma>\<rfloor>\<^sub>S\<^sub>A\<^sub>B\<^sub>R\<rfloor>\<^sub>s"
-
-subsection {*UTP-Relations lift and drop*}
-
-abbreviation lift_rel_uexpr_cpa ("\<lceil>_\<rceil>\<^sub>A\<^sub>B\<^sub>R")
-where "\<lceil>P\<rceil>\<^sub>A\<^sub>B\<^sub>R \<equiv> P \<oplus>\<^sub>p (\<Sigma>\<^sub>A\<^sub>B\<^sub>R \<times>\<^sub>L \<Sigma>\<^sub>A\<^sub>B\<^sub>R)"
-
-abbreviation lift_pre_uexpr_cpa ("\<lceil>_\<rceil>\<^sub>A\<^sub>B\<^sub>R\<^sub><")
-where "\<lceil>p\<rceil>\<^sub>A\<^sub>B\<^sub>R\<^sub>< \<equiv> \<lceil>\<lceil>p\<rceil>\<^sub><\<rceil>\<^sub>A\<^sub>B\<^sub>R"
-
-abbreviation lift_post_uexpr_cpa ("\<lceil>_\<rceil>\<^sub>A\<^sub>B\<^sub>R\<^sub>>")
-where "\<lceil>p\<rceil>\<^sub>A\<^sub>B\<^sub>R\<^sub>> \<equiv> \<lceil>\<lceil>p\<rceil>\<^sub>>\<rceil>\<^sub>A\<^sub>B\<^sub>R"
-
-abbreviation drop_cpa_rel_uexpr ("\<lfloor>_\<rfloor>\<^sub>A\<^sub>B\<^sub>R")
-where "\<lfloor>P\<rfloor>\<^sub>A\<^sub>B\<^sub>R \<equiv> P \<restriction>\<^sub>p (\<Sigma>\<^sub>A\<^sub>B\<^sub>R \<times>\<^sub>L \<Sigma>\<^sub>A\<^sub>B\<^sub>R)"
-
-abbreviation drop_cpa_pre_uexpr ("\<lfloor>_\<rfloor>\<^sub><\<^sub>A\<^sub>B\<^sub>R")
-where "\<lfloor>P\<rfloor>\<^sub><\<^sub>A\<^sub>B\<^sub>R \<equiv> \<lfloor>\<lfloor>P\<rfloor>\<^sub>A\<^sub>B\<^sub>R\<rfloor>\<^sub><"
-
-abbreviation drop_cpa_post_uexpr ("\<lfloor>_\<rfloor>\<^sub>>\<^sub>A\<^sub>B\<^sub>R")
-where "\<lfloor>P\<rfloor>\<^sub>>\<^sub>A\<^sub>B\<^sub>R \<equiv> \<lfloor>\<lfloor>P\<rfloor>\<^sub>A\<^sub>B\<^sub>R\<rfloor>\<^sub>>"
-
-subsection {* Reactive lemmas *}
-
-
-subsection{*Healthiness conditions*}
-
-text {*Programs in abrupt state do not progress*}   
-term "\<lceil>p\<rceil>\<^sub>A\<^sub>B\<^sub>R" 
-term "SKIP"
-find_theorems "\<Sigma>\<^sub>D"  
-term " \<lparr>lens_get = des_vars.more,
-       lens_put = \<lambda>\<sigma> u. \<sigma>\<lparr>des_vars.more := u\<rparr>\<rparr>"
-
-
-term "des_vars.more"  
-term " \<lparr>lens_get = des_vars.more,
-       lens_put = \<lambda>\<sigma> u. undefined\<rparr>"   
-term "\<lbrakk>v\<rbrakk>\<^sub>e ((abr_vars.more \<circ> des_vars.more) s)"
-term "\<lbrakk>v\<rbrakk>\<^sub>e"  
-term "abr_vars.more"  
-term "des_vars.more"
-term "Rep_uexpr o Rep_prog  "
-term "Abs_prog  o Abs_uexpr "  
-term "Abs_prog o des_vars.more "
-term "Rep_prog "
-term "Abs_prog"  
-term "Abs_prog o abr_vars.more "
-term "Rep_prog o abr_vars.more "  
-term "abr_vars.more "
-  
-definition abrh_def [upred_defs]: 
-  "abrh(P) = (IF &abrupt THEN SKIP ELSE  P FI)"
-
-section{*Control flow statements*}
-
-subsection{*SKIP*}
-definition  
-skip_abr_def [urel_defs]: "skip_abr=  abrh(SKIP)"
-
-subsection{*Assign*}
-
-definition  
-assigns_abr_def [urel_defs]: "assigns_abr \<sigma> =  abrh(\<langle>\<sigma>\<rangle>\<^sub>p)"
-
-subsection{*Throw*}
-
-definition  
-throw_abr_def [urel_defs]: "throw_abr  =  assigns_abr [&abrupt \<mapsto>\<^sub>s true]"
-
-subsection{*Sequential composition*}
-text {*It does not need a definition. We get it by type inference.*}  
-term "(throw_abr) ; (p )"  
-subsection{*Conditional composition*}
-
-definition  
-if_abr_def [urel_defs]: "if_abr b P Q  =  IF (b \<oplus>\<^sub>p \<Sigma>\<^sub>A\<^sub>B\<^sub>R) THEN P ELSE Q FI"
-
-subsection{*Iterations*}
-
-definition  
-while_abr_def [urel_defs]: "while_abr b I C  =  WHILE (b \<oplus>\<^sub>p \<Sigma>\<^sub>A\<^sub>B\<^sub>R) \<and> \<not>&abrupt INVR I DO C OD"
-
-subsection{*Recursion*}
-(*TODO @Yakoub*)
-  
-section {*algebraic laws*} 
-
-lemma [Algebraic_Laws_prog]:"IF b THEN P ELSE P FI = P"
-  by (simp add: prog_rep_eq Algebraic_Laws.cond_idem)
-
-lemma [Algebraic_Laws_prog]:"skip_abr ;  P =  P" "P ; skip_abr = P"
-  unfolding skip_abr_def abrh_def
-  by (simp add: Algebraic_Laws_prog)+  
-
-lemma [Algebraic_Laws_prog]:"throw_abr ;  (abrh P) = throw_abr"     
-  unfolding throw_abr_def abrh_def assigns_abr_def skip_abr_def
-  apply (simp add: prog_rep_eq) 
-   apply rel_auto
-  done
-
-lemma "(abrh P) ;  \<langle>[&abrupt \<mapsto>\<^sub>s true]\<rangle>\<^sub>p = (abrh P)"
-    unfolding throw_abr_def abrh_def assigns_abr_def skip_abr_def
-    apply (simp add: prog_rep_eq) 
-      
-    apply rel_simp
-    apply transfer
-    unfolding Healthy_def H1_def H3_def
-    apply rel_simp
-      apply auto
-    apply metis
-          apply metis
-         apply metis
-        apply metis
-
-    oops
-lemma "abrh(\<langle>a\<rangle>\<^sub>p) ; abrh (throw_abr ;  IF &abrupt THEN (abrupt:== (\<not> &abrupt) ; abrh(\<langle>b\<rangle>\<^sub>p)) ELSE skip_abr FI) = 
-         (abrh(\<langle>a\<rangle>\<^sub>p); abrh(\<langle>b\<rangle>\<^sub>p))"
-  unfolding throw_abr_def abrh_def assigns_abr_def skip_abr_def
-    apply (simp add: prog_rep_eq) 
-  apply rel_auto
-  apply (smt abr_vars.ext_inject abr_vars_ext_def)+
-  done  
- 
-lemma "abrh(P) ; abrh (throw_abr ;  IF &abrupt THEN (abrupt:== (\<not> &abrupt) ; abrh(Q)) ELSE skip_abr FI) = 
-         (abrh(P); abrh(Q))"
-  unfolding throw_abr_def abrh_def assigns_abr_def skip_abr_def
-    apply (simp add: prog_rep_eq) 
-  apply rel_auto
-  apply transfer
-  unfolding Healthy_def H1_def H3_def
-    apply rel_simp
-         apply blast
-      apply transfer
-    unfolding Healthy_def H1_def H3_def
-    apply rel_simp
-          apply blast
-      apply transfer
-    unfolding Healthy_def H1_def H3_def
-    apply rel_simp
-         apply blast
-      apply transfer
-    unfolding Healthy_def H1_def H3_def
-    apply rel_simp
-    apply metis
-   apply transfer
-    unfolding Healthy_def H1_def H3_def
-    apply rel_simp
-       apply metis
-      apply transfer
-    unfolding Healthy_def H1_def H3_def
-    apply rel_simp
-      apply metis
-      apply transfer
-    unfolding Healthy_def H1_def H3_def
-    apply rel_simp
-     apply metis
-    apply (smt abr_vars.select_convs(2))
-done
 end
