C-verifier/src/Midend-IVL/Isabelle-UTP-Extended/impl/utp_prog_abrupt_more.thy
@@ -1,0 +1,203 @@
+section {* Imperative Programs *}
+  
+theory utp_prog_abrupt_more
+  imports 
+    "../hoare/HoareLogic/TotalCorrectness/IMP_Prog/utp_hoare_ndes_prog"
+begin
+
+section {*Abrupt*}
+subsection {*Sequential C-program alphabet*}
+
+text 
+{* In order to capture exceptions, we extend the alphabet of UTP by an additional global 
+   state variables:
+   \begin{itemize}   
+      \<^item> abrupt: a boolean variable used to specify if the program is in an abrupt state or not.
+   \end{itemize}
+*}
+
+alphabet abr_vars = 
+  abrupt :: bool
+
+declare  abr_vars.splits [alpha_splits]
+  
+subsubsection {*Alphabet proofs*}
+text {*
+  The two locale interpretations below are a technicality to improve automatic
+  proof support via the predicate and relational tactics. This is to enable the
+  (re-)interpretation of state spaces to remove any occurrences of lens types
+  after the proof tactics @{method pred_simp} and @{method rel_simp}, or any
+  of their derivatives have been applied. Eventually, it would be desirable to
+  automate both interpretations as part of a custom outer command for defining
+  alphabets.
+*}
+
+interpretation cp_abr:
+  lens_interp "\<lambda> (ok, r) . (ok, abrupt\<^sub>v r, more r)"
+apply (unfold_locales)
+apply (rule injI)
+apply (clarsimp)
+done
+
+interpretation cp_abr_rel: lens_interp "\<lambda>(ok, ok', r, r').
+  (ok, ok', abrupt\<^sub>v r, abrupt\<^sub>v r', more r, more r')"
+apply (unfold_locales)
+apply (rule injI)
+apply (clarsimp)
+done
+
+subsubsection {*Type lifting*}
+
+type_synonym '\<alpha> hrel_abr_des  = "'\<alpha> abr_vars_scheme prog"
+
+subsubsection {*Syntactic type setup*}
+
+notation abr_vars_child_lens ("\<Sigma>\<^sub>A\<^sub>B\<^sub>R")
+
+syntax
+  "_svid_st_alpha"  :: "svid" ("\<Sigma>\<^sub>A\<^sub>B\<^sub>R")
+translations
+  "_svid_st_alpha" => "CONST abr_vars_child_lens"
+
+subsection {*Substitution lift and drop*}
+
+abbreviation lift_rel_usubst_cpa ("\<lceil>_\<rceil>\<^sub>S\<^sub>A\<^sub>B\<^sub>R")
+where "\<lceil>\<sigma>\<rceil>\<^sub>S\<^sub>A\<^sub>B\<^sub>R \<equiv> \<sigma> \<oplus>\<^sub>s (\<Sigma>\<^sub>A\<^sub>B\<^sub>R \<times>\<^sub>L \<Sigma>\<^sub>A\<^sub>B\<^sub>R)"
+
+abbreviation lift_usubst_cpa ("\<lceil>_\<rceil>\<^sub>s\<^sub>A\<^sub>B\<^sub>R")
+where "\<lceil>\<sigma>\<rceil>\<^sub>s\<^sub>A\<^sub>B\<^sub>R \<equiv> \<lceil>\<lceil>\<sigma>\<rceil>\<^sub>s\<rceil>\<^sub>S\<^sub>A\<^sub>B\<^sub>R"
+
+abbreviation drop_cpa_rel_usubst ("\<lfloor>_\<rfloor>\<^sub>S\<^sub>A\<^sub>B\<^sub>R")
+where "\<lfloor>\<sigma>\<rfloor>\<^sub>S\<^sub>A\<^sub>B\<^sub>R \<equiv> \<sigma> \<restriction>\<^sub>s (\<Sigma>\<^sub>A\<^sub>B\<^sub>R \<times>\<^sub>L \<Sigma>\<^sub>A\<^sub>B\<^sub>R)"
+
+abbreviation drop_cpa_usubst ("\<lfloor>_\<rfloor>\<^sub>s\<^sub>A\<^sub>B\<^sub>R")
+where "\<lfloor>\<sigma>\<rfloor>\<^sub>s\<^sub>A\<^sub>B\<^sub>R \<equiv> \<lfloor>\<lfloor>\<sigma>\<rfloor>\<^sub>S\<^sub>A\<^sub>B\<^sub>R\<rfloor>\<^sub>s"
+
+subsection {*UTP-Relations lift and drop*}
+
+abbreviation lift_rel_uexpr_cpa ("\<lceil>_\<rceil>\<^sub>A\<^sub>B\<^sub>R")
+where "\<lceil>P\<rceil>\<^sub>A\<^sub>B\<^sub>R \<equiv> P \<oplus>\<^sub>p (\<Sigma>\<^sub>A\<^sub>B\<^sub>R \<times>\<^sub>L \<Sigma>\<^sub>A\<^sub>B\<^sub>R)"
+
+abbreviation lift_pre_uexpr_cpa ("\<lceil>_\<rceil>\<^sub>A\<^sub>B\<^sub>R\<^sub><")
+where "\<lceil>p\<rceil>\<^sub>A\<^sub>B\<^sub>R\<^sub>< \<equiv> \<lceil>\<lceil>p\<rceil>\<^sub><\<rceil>\<^sub>A\<^sub>B\<^sub>R"
+
+abbreviation lift_post_uexpr_cpa ("\<lceil>_\<rceil>\<^sub>A\<^sub>B\<^sub>R\<^sub>>")
+where "\<lceil>p\<rceil>\<^sub>A\<^sub>B\<^sub>R\<^sub>> \<equiv> \<lceil>\<lceil>p\<rceil>\<^sub>>\<rceil>\<^sub>A\<^sub>B\<^sub>R"
+
+abbreviation drop_cpa_rel_uexpr ("\<lfloor>_\<rfloor>\<^sub>A\<^sub>B\<^sub>R")
+where "\<lfloor>P\<rfloor>\<^sub>A\<^sub>B\<^sub>R \<equiv> P \<restriction>\<^sub>p (\<Sigma>\<^sub>A\<^sub>B\<^sub>R \<times>\<^sub>L \<Sigma>\<^sub>A\<^sub>B\<^sub>R)"
+
+abbreviation drop_cpa_pre_uexpr ("\<lfloor>_\<rfloor>\<^sub><\<^sub>A\<^sub>B\<^sub>R")
+where "\<lfloor>P\<rfloor>\<^sub><\<^sub>A\<^sub>B\<^sub>R \<equiv> \<lfloor>\<lfloor>P\<rfloor>\<^sub>A\<^sub>B\<^sub>R\<rfloor>\<^sub><"
+
+abbreviation drop_cpa_post_uexpr ("\<lfloor>_\<rfloor>\<^sub>>\<^sub>A\<^sub>B\<^sub>R")
+where "\<lfloor>P\<rfloor>\<^sub>>\<^sub>A\<^sub>B\<^sub>R \<equiv> \<lfloor>\<lfloor>P\<rfloor>\<^sub>A\<^sub>B\<^sub>R\<rfloor>\<^sub>>"
+
+subsection {* Reactive lemmas *}
+
+
+subsection{*Healthiness conditions*}
+  
+definition abrh_def [upred_defs]: 
+  "abrh(P) = (IF &abrupt THEN SKIP ELSE  P FI)"
+
+section{*Control flow statements*}
+
+subsection{*SKIP*}
+definition  
+skip_abr_def [urel_defs]: "skip_abr=  abrh(SKIP)"
+
+subsection{*Assign*}
+
+definition  
+assigns_abr_def [urel_defs]: "assigns_abr \<sigma> =  abrh(\<langle>\<sigma>\<rangle>\<^sub>p)"
+
+subsection{*Throw*}
+
+definition  
+throw_abr_def [urel_defs]: "throw_abr  =  assigns_abr [&abrupt \<mapsto>\<^sub>s true]"
+
+subsection{*Sequential composition*}
+text {*It does not need a definition. We get it by type inference.*}  
+term "(throw_abr) ; (p )"  
+subsection{*Conditional composition*}
+
+definition  
+if_abr_def [urel_defs]: "if_abr b P Q  =  IF (b \<oplus>\<^sub>p \<Sigma>\<^sub>A\<^sub>B\<^sub>R) THEN P ELSE Q FI"
+
+subsection{*Iterations*}
+
+definition  
+while_abr_def [urel_defs]: "while_abr b I C  = INVR I  WHILE (b \<oplus>\<^sub>p \<Sigma>\<^sub>A\<^sub>B\<^sub>R) \<and> \<not>&abrupt DO C OD"
+
+subsection{*Recursion*}
+(*TODO @Yakoub*)
+
+definition mu_abr_def [urel_defs]:
+  "mu_abr P = (\<mu>\<^sub>p X \<bullet> P (abrh X))"
+  
+subsection {*Try catch*}
+
+definition  try_catch_abr_def [urel_defs]:
+  "try_catch_abr P Q = 
+   abrh (P ;  IF &abrupt THEN (abrupt:== (\<not> &abrupt) ; abrh(Q)) ELSE skip_abr FI)"
+
+section {*algebraic laws*} 
+
+lemma [algebraic_laws_prog]:"IF b THEN P ELSE P FI = P"
+  by (simp add: prog_rep_eq Algebraic_Laws.cond_idem)
+
+lemma [algebraic_laws_prog]:"skip_abr ;  P =  P" "P ; skip_abr = P"
+  unfolding skip_abr_def abrh_def
+  by (simp add: algebraic_laws_prog)+  
+
+lemma [algebraic_laws_prog]:"throw_abr ;  (abrh P) = throw_abr"     
+  unfolding throw_abr_def abrh_def assigns_abr_def skip_abr_def
+  apply (simp add: prog_rep_eq) 
+   apply rel_auto
+  done
+
+lemma "abrh(\<langle>a\<rangle>\<^sub>p) ; abrh (throw_abr ;  IF &abrupt THEN (abrupt:== (\<not> &abrupt) ; abrh(\<langle>b\<rangle>\<^sub>p)) ELSE skip_abr FI) = 
+         (abrh(\<langle>a\<rangle>\<^sub>p); abrh(\<langle>b\<rangle>\<^sub>p))"
+  unfolding throw_abr_def abrh_def assigns_abr_def skip_abr_def
+    apply (simp add: prog_rep_eq) 
+  apply rel_auto
+  apply (smt abr_vars.ext_inject abr_vars_ext_def)+
+  done  
+ 
+lemma "abrh(P) ; abrh (throw_abr ;  IF &abrupt THEN (abrupt:== (\<not> &abrupt) ; abrh(Q)) ELSE skip_abr FI) = 
+         (abrh(P); abrh(Q))"
+  unfolding throw_abr_def abrh_def assigns_abr_def skip_abr_def
+    apply (simp add: prog_rep_eq) 
+  apply rel_auto
+  apply transfer
+  unfolding Healthy_def H1_def H3_def
+    apply rel_simp
+         apply blast
+      apply transfer
+    unfolding Healthy_def H1_def H3_def
+    apply rel_simp
+          apply blast
+      apply transfer
+    unfolding Healthy_def H1_def H3_def
+    apply rel_simp
+         apply blast
+      apply transfer
+    unfolding Healthy_def H1_def H3_def
+    apply rel_simp
+    apply metis
+   apply transfer
+    unfolding Healthy_def H1_def H3_def
+    apply rel_simp
+       apply metis
+      apply transfer
+    unfolding Healthy_def H1_def H3_def
+    apply rel_simp
+      apply metis
+      apply transfer
+    unfolding Healthy_def H1_def H3_def
+    apply rel_simp
+     apply metis
+    apply (smt abr_vars.select_convs(2))
+done 
+end
