C-verifier/src/Midend-IVL/Isabelle-UTP-Extended/utp/utp_rec_total_des.thy
@@ -113,30 +113,30 @@ proof -
   thus ?thesis
     by pred_simp
 qed    
-    
+  
 lemma ndesign_mu_wf_refine_intro: 
   assumes   WF: "wf R"
     and      M: "Mono\<^bsub>uthy_order NDES\<^esub> B"
     and      H: "B \<in> \<lbrakk>\<^bold>N\<rbrakk>\<^sub>H \<rightarrow> \<lbrakk>\<^bold>N\<rbrakk>\<^sub>H"
     and  induct_step:
-    "\<And>st. ((Pre \<and> E =\<^sub>u \<guillemotleft>st\<guillemotright>) \<turnstile>\<^sub>n Post) \<sqsubseteq> (B ((Pre \<and> (E,\<guillemotleft>st\<guillemotright>)\<^sub>u\<in>\<^sub>u\<guillemotleft>R\<guillemotright>) \<turnstile>\<^sub>n Post))"
+    "\<And>e. ((Pre \<and> E =\<^sub>u \<guillemotleft>e\<guillemotright>) \<turnstile>\<^sub>n Post) \<sqsubseteq> (B ((Pre \<and> (E,\<guillemotleft>e\<guillemotright>)\<^sub>u\<in>\<^sub>u\<guillemotleft>R\<guillemotright>) \<turnstile>\<^sub>n Post))"
   shows "(Pre \<turnstile>\<^sub>n Post) \<sqsubseteq> \<mu>\<^sub>N B"            
 proof -          
   {
-  fix st
-  have "(Pre \<and> E =\<^sub>u \<guillemotleft>st\<guillemotright>) \<turnstile>\<^sub>n Post \<sqsubseteq> \<mu>\<^sub>N B" 
+  fix e
+  have "(Pre \<and> E =\<^sub>u \<guillemotleft>e\<guillemotright>) \<turnstile>\<^sub>n Post \<sqsubseteq> \<mu>\<^sub>N B" 
     using WF proof (induction rule: wf_induct_rule)
-    case (less st)
-    hence 0: "(Pre \<and> (E, \<guillemotleft>st\<guillemotright>)\<^sub>u \<in>\<^sub>u \<guillemotleft>R\<guillemotright>) \<turnstile>\<^sub>n Post \<sqsubseteq> \<mu>\<^sub>N B"
+    case (less e)
+    hence 0: "(Pre \<and> (E, \<guillemotleft>e\<guillemotright>)\<^sub>u \<in>\<^sub>u \<guillemotleft>R\<guillemotright>) \<turnstile>\<^sub>n Post \<sqsubseteq> \<mu>\<^sub>N B"
       by rel_blast
     from M H normal_design_theory_continuous.LFP_lemma3 mono_Monotone_utp_order
     have 1: "\<mu>\<^sub>N B \<sqsubseteq>  B (\<mu>\<^sub>N B)"
       by blast
-    from 0 1 have 2:"(Pre \<and> (E,\<guillemotleft>st\<guillemotright>)\<^sub>u\<in>\<^sub>u\<guillemotleft>R\<guillemotright>) \<turnstile>\<^sub>n Post \<sqsubseteq> B (\<mu>\<^sub>N B)"
+    from 0 1 have 2:"(Pre \<and> (E,\<guillemotleft>e\<guillemotright>)\<^sub>u\<in>\<^sub>u\<guillemotleft>R\<guillemotright>) \<turnstile>\<^sub>n Post \<sqsubseteq> B (\<mu>\<^sub>N B)"
       by simp
-    have 3: "B ((Pre \<and> (E, \<guillemotleft>st\<guillemotright>)\<^sub>u \<in>\<^sub>u \<guillemotleft>R\<guillemotright>) \<turnstile>\<^sub>n Post) \<sqsubseteq> B (\<mu>\<^sub>N B)"
+    have 3: "B ((Pre \<and> (E, \<guillemotleft>e\<guillemotright>)\<^sub>u \<in>\<^sub>u \<guillemotleft>R\<guillemotright>) \<turnstile>\<^sub>n Post) \<sqsubseteq> B (\<mu>\<^sub>N B)"
       by (auto intro: Mono_utp_orderD M 0)
-    have 4:"(Pre \<and> E =\<^sub>u \<guillemotleft>st\<guillemotright>) \<turnstile>\<^sub>n Post \<sqsubseteq> \<dots>" 
+    have 4:"(Pre \<and> E =\<^sub>u \<guillemotleft>e\<guillemotright>) \<turnstile>\<^sub>n Post \<sqsubseteq> \<dots>" 
       by (rule induct_step)
     show ?case
       using order_trans[OF 3 4] H M normal_design_theory_continuous.LFP_lemma2 dual_order.trans mono_Monotone_utp_order 
